Work on subst lang. Implement better script for automatic lang checking

src/langs/Subst.v
@@ -56,7 +56,35 @@ Ltac recognize_lang :=
     |- wf_lang ?L =>
     suff: type_wf_lang L = Some tt;
     [ by apply type_wf_lang_recognizes
-    | by compute]
+    | by cbv]
+  end.
+
+Ltac recognize_ctx :=  match goal with
+    |- wf_ctx ?L ?C =>
+    suff: type_wf_ctx L C = Some tt;
+    [ apply type_wf_ctx_recognizes
+    | by cbv]
+  end.
+
+Ltac recognize_sort :=  match goal with
+    |- wf_sort ?L ?C ?T =>
+    suff: type_wf_sort L C T = Some tt;
+    [ apply type_wf_sort_recognizes
+    | by cbv]
+  end.
+
+Ltac recognize_term :=  match goal with
+    |- wf_term ?L ?C ?E ?T =>
+    suff: type_wf_term L C E = Some T;
+    [ apply type_wf_term_recognizes
+    | by cbv]
+  end.
+
+Ltac recognize_subst :=  match goal with
+    |- wf_subst ?L ?C ?S ?C' =>
+    suff: type_wf_subst L C S C' = Some tt;
+    [ apply type_wf_subst_recognizes
+    | by cbv]
   end.
 
 Ltac recognize_rule' :=
@@ -69,7 +97,15 @@ Ltac recognize_rule' :=
 Lemma cat_stx_wf : wf_lang cat_stx.
 Proof using . recognize_lang. Qed.
 
+(* TODO: put coercion, hint in right places *)
 Coercion var : nat >-> exp.
+
+Hint Resolve type_wf_lang_recognizes : judgment.
+Hint Resolve type_wf_rule_recognizes : judgment.
+Hint Resolve type_wf_ctx_recognizes : judgment.
+Hint Resolve type_wf_sort_recognizes : judgment.
+Hint Resolve type_wf_term_recognizes : judgment.
+Hint Resolve type_wf_subst_recognizes : judgment.
 
 Definition cat_lang : lang :=
   (* compose associativity *)
@@ -91,326 +127,107 @@ Definition cat_lang : lang :=
 
 Lemma cat_lang_wf : wf_lang cat_lang.
 Proof using .
-  recognize_lang.
+  auto with judgment.
+  (*recognize_lang.*)
 Qed.
+(*TODO: symmetry for rules;currently only go one direction *)
 
-Lemma wf_ob c : wf_ctx cat_stx c -> wf_sort cat_stx c ob.
+
+Lemma wf_ob c : wf_ctx cat_lang c -> wf_sort cat_lang c ob.
 Proof using .
-  intros.
-  suff: type_wf_sort cat_stx c ob = Some tt; first by apply type_wf_sort_recognizes.
-  by compute.
+  auto with judgment.
 Qed.
 
+Definition ty a := con 7 [:: a].
+Definition ty_subst a b s t := con 8 [:: t; s; b; a].
+Definition el a t := con 9 [:: t; a].
+Definition el_subst a b s t m := con 10 [:: m; t; s; b; a].
 
-(* TODO: need decision instead of recognizer for this one  due to a, b*)
-Lemma wf_hom c a b : wf_term cat_stx c a ob -> wf_term cat_stx c b ob -> wf_sort cat_stx c (hom a b).
-Proof.
-  intros.
-  suff: type_wf_sort cat_stx c (hom a b) = Some tt; first by apply type_wf_sort_recognizes; eauto with judgment.
-  
-  compute.
-Qed.
+Definition emp := con 15 [::].
+Definition forget a := con 16 [:: a].
 
-  easy_wf_lang; auto.
-  constructor; eauto.
-  easy_wf_lang; eauto.
-  easy_wf_lang; eauto.
-  eapply wf_to_ctx; eauto.
-  solve_easy_wf.
-  solve_easy_wf.
-Qed.
+Definition ext g a := con 19 [:: a; g] (*[:: ty 0; ob]*).
+Definition snoc a b t g n := con 20 [:: n; g; t; b; a]
+(*[:: el 0 (ty_subst 0 1 3 2); hom 0 1; ty 1; ob; ob]*).
+Definition p a t := con 21 [:: t; a].
+Definition q a t := con 22 [:: t; a].
 
-Lemma wf_id c a : wf_term cat_stx c a ob -> wf_term cat_stx c (id a) (hom a a).
-Proof.
-  intro.
-  change (hom a a) with (hom (var 0) (var 0))[/[::a]/].
-  easy_wf_lang.
-  constructor.
-  easy_wf_lang.
-  eapply wf_to_ctx; eauto.
-  solve_easy_wf.
-  easy_wf_lang.
-  apply: le_sort_refl.
-  solve_easy_wf.
-  apply: wf_term_sort; eauto.
-Qed.
+Definition subst_lang : lang :=
+  (term_rule [:: ty 0; ob]
+             (el (ext 0 1)
+                 (ty_subst  (ext 0 1) 0 (p 0 1) 1)))::
+  (term_rule [:: ty 0; ob] (hom (ext 0 1) 0))::
+  (term_rule [:: el 0 (ty_subst 0 1 3 2); hom 0 1; ty 1; ob; ob]
+             (hom 0 (ext 1 2)))::
+  (term_rule [:: ty 0; ob] ob)::
+  (term_le [::] (id emp) (forget emp) (hom emp emp))::
+  (term_le [:: hom 0 1; ob; ob] (cmp 0 1 emp (forget 1) 2) (forget 0) (hom 0 emp))::
+  (term_rule [:: ob] (hom 0 emp))::
+  (term_rule [::] ob)::
+  (* el_subst compose to sequence *)
+  (term_le [:: ty 2; hom 1 2; hom 0 1; ob; ob; ob]
+           (ty_subst 0 2 (cmp 0 1 2 4 3) 5)
+           (ty_subst 0 1 3 (ty_subst 1 2 4 5))
+           (ty 0))::
+  (* id el_subst; may be the first rule that holds, but isn't recognized. *)
+  (term_le [:: el 0 1; ty 0; ob] (el_subst 0 0 (id 0) 1 2) 2 (el 0 1))::
+  (* ty_subst compose to sequence *)
+  (term_le [:: ty 2; hom 1 2; hom 0 1; ob; ob; ob]
+           (ty_subst 0 2 (cmp 0 1 2 4 3) 5)
+           (ty_subst 0 1 3 (ty_subst 1 2 4 5))
+           (ty 0))::
+  (* id ty_subst *)
+  (term_le [:: ty 0; ob] (ty_subst 0 0 (id 0) 1) 1 (ty 0))::
+  (term_rule [:: el 1 3; ty 1; hom 0 1; ob; ob] (el 0 (ty_subst 0 1 2 3)))::
+  (sort_rule [:: ty 0; ob])::
+  (term_rule [:: ty 1; hom 0 1; ob; ob] (ty 0))::
+  (sort_rule [:: ob])::cat_lang.
 
-(*
-Lemma wf_hom_inversion c A B
-  : wf_sort cat_stx c (hom A B) ->
-    wf_term cat_stx c A ob /\ wf_term cat_stx c B ob.
-Proof.
-  inversion.
-  move: H4.
-  unfold is_nth.
-  simpl.
-  change (3+0) with 3.
-  move /eqP.
-  case => c'eq.
-  move: H5.
-  rewrite -c'eq.
-  inversion.
-  split; eauto.
-  inversion H10.
-  eauto.
-Qed.*)
-
-
-(* TODO: move to exp,core *)
-
-Scheme wf_sort_subst_props_ind := Minimality for wf_sort Sort Prop
-  with wf_subst_subst_props_ind := Minimality for wf_subst Sort Prop
-  with wf_term_subst_props_ind := Minimality for wf_term Sort Prop.
-
-Combined Scheme subst_props_ind from
-         wf_sort_subst_props_ind,
-wf_subst_subst_props_ind,
-wf_term_subst_props_ind.
-(*TODO: will eventually want a library of betterinduction schemes for same reason I wantedparameters*)
-
-(* TODO: move to utils*)
-Lemma nth_error_size_lt {A} (l : seq A) n e : List.nth_error l n = Some e -> n < size l.
-Proof.
-  elim: n l => [| n IH];case; simpl; auto; try done.
-Qed.
-
-Lemma le_ctx_len_eq  l c c' : le_ctx l c c' -> size c = size c'
-with le_sort_ctx_len_eq l c c' t t' : le_sort l c c' t t' -> size c = size c'.
-Proof.
-  case; simpl; auto; intros; f_equal.
-  apply: le_sort_ctx_len_eq; eauto.
-  intro les.
-  eapply wf_to_ctx in les.
-  apply: le_ctx_len_eq; eauto.
-TODO: get a nicer induction w/ presuppositions
-  
-Lemma wf_is_ws : (forall l c t, wf_sort l c t -> ws_exp (size c) t)
-                 /\ (forall l c s c', wf_subst l c s c' -> ws_subst (size c) s)
-                 /\ (forall l c e t, wf_term l c e t -> ws_exp (size c) e).
-Proof.
-  apply: subst_props_ind; simpl; intros; try apply /andP; auto; try apply: nth_error_size_lt; eauto.
-  eapply wf_to_ctx in H1.
-  TODO: show cssame size
-Qed.
-
-
-Lemma wf_subst_props c s
-  : (forall l c' t, wf_sort l c' t -> wf_subst l c s c' -> wf_sort l c t[/s/])
-    /\ (forall l c' s2 c2', wf_subst l c' s2 c2' -> wf_subst l c s c' -> wf_subst l c (subst_cmp s2 s) c2')
-    /\ (forall l c' e t, wf_term l c' e t -> wf_subst l c s c' -> wf_term l c e[/s/] t[/s/]).
-Proof.
-  apply: subst_props_ind.
-  {  
-    intros.
-    rewrite con_subst_cmp.
-    eauto.
-  }
-  {
-    intros; simpl; constructor.
-    by apply wf_to_ctx in H0.
-  }
-  {
-    intros; simpl; constructor; eauto.
-    rewrite sep_subst_cmp.
-    auto.
-    Search _ ws_subst.
-    TODO: need wf ->ws
-
-    
-  
-Lemma wf_cmp c A B C g f
-  : wf_term cat_stx c f (hom A B) ->
-    wf_term cat_stx c g (hom B C) ->
-    wf_term cat_stx c (cmp A B C g f) (hom A C).
-Proof.
-  intros.
-  eapply wf_term_subst.
-  change (hom A C) with (hom (var 4) (var 2)) [/[:: f; g; C; B; A]/].
-  eapply wf_term_by.
-  2:{
-    easy_wf_lang; eauto.
-    constructor; eauto.
-    repeat easy_wf_lang; eauto.
-    
-  easy_wf_lang.
-  easy_wf_lang.
-  eapply wf_to_ctx; eauto
-  
-Goal wf_term cat_stx [:: ob]
-     (cmp (var 0) (var 0) (var 0) (id (var 0)) (id (var 0))) (hom (var 0) (var 0)).
-Proof.
-  change (hom (var 0) (var 0)) with (hom (var 2) (var 3))[/[:: id (var 0); id (var 0); var 0; var 0; var 0]/].
-  eapply wf_term_by.
-  compute.
-  match goal with
-  | |- wf_term ?l ?c (con ?m ?s) [?n|] =>
-    change (wf_term l c (con m s) [n|])
-      with (wf_term l c (con m s) [n|][/s/])
+(*TODO: move to utils *)
+Ltac unfold_tail l :=
+  match l with
+  | _::?l' => unfold_tail l'
+  | _ => unfold l
   end.
-  
 
-Definition cat_lang' : seq named_rule :=
-  [:: {<n 
-  ]++cat_stx'.
+(* TODO: move to EasyWF*)
+Ltac wf_lang_eauto :=
+   repeat match goal with
+          | |- wf_lang ?l => unfold_tail l
+         end;
+  repeat match goal with
+         | |- wf_lang (?R :: ?L) =>
+           suff: wf_lang L;
+             [intro;
+              apply: wf_lang_cons;
+              eauto with judgment|]
+         | |- wf_lang nil => apply: wf_lang_nil
+         end.
 
-           
-
-Definition ctx_lang : lang :=
-  [:: {| [:: [2(*tp*)|]; [1(*ctx*)|]] |- (*C,t*) [1(*ctx*)|]};
-     {| [::] |- (*.*) [0 (*ctx*)|]};
-     {| [::] |- (*ctx*) sort };
-     {| [::] |- (*tp*) sort }].
-
-Lemma wf_ctx_lang : wf_lang ctx_lang.
-Proof.
-  pose p := eqP.
-  repeat easy_wf_lang.
-Qed.  
-
-Definition subst_lang' : lang :=
-  [::
-    (* {| [:: [5(*tp*)|];[1(*var*)| var 1; var 0];[5(*tp*)|]; [4(*ctx*)|]]
-        |- (*S x*) [1(*var*)| [2(*C,t'*)| var 3; var 0];var 2]};
-     *){| [:: [4(*tp*)|]; [3(*ctx*)|]] |- (*Z*) [0(*var*)| var 0; [1(*C,t*)| var 0; var 1]]};
-     {| [:: [3(*tp*)|]; [2(*ctx*)|]] |- (*var(C|-t)*) sort}]
-++ ctx_lang.
-(* TODO: substitutions, judgments, equalities *)
-
-
-Lemma wf_subst_lang : wf_lang subst_lang'.
-Proof.
-  pose p := eqP.
-  pose cl := wf_ctx_lang.
-  repeat easy_wf_lang.
-  change [3|] with [3|][/[:: var 0; var 1]/].  
-  apply: wf_term_by.
-  unfold is_nth; simpl.
-  compute_adds.
-  apply /eqP; f_equal.
-  repeat easy_wf_lang.
+Lemma subst_lang_wf : wf_lang subst_lang.
+Proof using .
+  wf_lang_eauto.
+  { (* element identity substitution *)
+    constructor;auto with judgment.     
+    apply: wf_term_conv.
+    1-3:auto with judgment.
+    instantiate (1:= el 0 (ty_subst 0 0 (id 0) 1)).
+    auto with judgment.
+    change (el 0 (ty_subst 0 0 (id 0) 1)) with (el 0 1)[/[:: (ty_subst 0 0 (id 0) 1); var 0]/].
+    change (el 0 1) at 3 with (el 0 1)[/[:: var 1; var 0]/].
+    eapply le_sort_subst'.
+    instantiate (1:=[:: ty 0; ob]).
+    2:eauto with judgment.
+    
+    eapply le_subst_cons'.
+    recognize_subst; eauto with judgment.
+    eapply le_subst_cons'.
+    recognize_subst; eauto with judgment.
+    eauto with judgment.
+    rewrite subst_nil.
+    eapply le_term_refl'; eauto with judgment.
+    change (ty 0) [/[:: var 0] /] with (ty 0).
+    change [:: el 0 1; ty 0; ob] with ([:: el 0 1] ++ [:: ty 0; ob]).
+    eapply mono_ctx; eauto with judgment.
+  }
 Qed.
-
-Definition subst_lang'' : lang :=
-  [:: {| [:: [5(*tp*)|];[1(*var*)| var 1; var 0];[4(*ctx*)|]; [5(*tp*)|]]
-        |- (*S x*) [1(*var*)| var 3 ; [2(*C,t'*)| var 0; var 2]]}]
-    ++ subst_lang'.
-
-Lemma wf_subst_lang'' : wf_lang subst_lang''.
-Proof.
-  pose wfp :=  wf_subst_lang.
-  repeat easy_wf_lang.
-  match goal with
-  | |- wf_term ?l ?c (con ?m ?s) [?n|] =>
-    change (wf_term l c (con m s) [n|])
-      with (wf_term l c (con m s) [n|][/s/])
-  end.
-  apply: wf_term_by.
-  unfold is_nth; simpl.
-  compute_adds.
-  eauto.
-  repeat easy_wf_lang.
-Qed.
-
-Definition subst_lang_syn : lang :=
-  [::{| [:: [4 | var 0; var 1] ; [3(*tp*)|]; [2(*ctx*)|]] |- [0| var 1; var 2]};
-     {| [:: [3(*tp*)|]; [2(*ctx*)|]] |- (*jdg(C|-t)*) sort}]
-    ++ subst_lang''.
-
-Lemma wf_syn : wf_lang subst_lang_syn
-
-  
-Definition subst_lang : lang subst_syn :=
-  (* terms *)
-  [::
-     (* ctxts*)
-     {| [::] |- empty_ctxt' .: ctxt'};
-     {| [:: term_var ctxt' ; term_var tp' ] |- cons_ctxt' (var 0) (var 1) .: ctxt'} ;
-     (* variables *)
-     {| [:: term_var tp'] |- zv' .: var_srt'(judg' (@! ,, (var 0)) (var 0))};
-     {| [:: term_var (var_srt' (judg' (var 0) (var 1))); term_var ctxt'; term_var tp']
-        |- (sv' (var 0)) .: var_srt' (judg' (@! ,, (var 0)) (var 0))};
-     (* judgments *)
-     {| [:: term_var (var 0); term_var (var_srt' (var 0)); sort_var]
-        |- (var 0) .: (var 2)}
-  ] ++
-    (* sorts *)
-    [:: {| [:: term_var ctxt' ; term_var tp' ] |- judg' (var 0) (var 1)} ;
-       {| [:: sort_var ] |- var_srt' (var 0)};
-       {| [::] |- ctxt' };
-       {| [::] |- tp' }
-    ].
-
-Definition list_syn : polynomial :=
-  [:: (unit, 0) (* nil *)
-   ; (unit, 2) (* cons*)].
-
-Definition subst_syn : polynomial :=
-  [:: (unit, 0) (* tp *)]
-    ++  [:: (unit, 0) (* ctxt *)]
-    ++ list_syn (* ctxt := . | ctxt, t:tp*)
-    ++ [:: (unit,2) (* jdg := ctxt |- t:tp *)]
-    ++ [:: (unit,0) ; (unit,1) (* var := 0 | S var*)]
-    ++ list_syn (* subst := . | subst, v:type*)
-    ++ [:: (unit,1) (*var := jdg*)].
-
-Definition tp {T} : constr subst_syn T := [{subst_syn,T}> 0 | tt, [*]].
-
-Definition ctxt {T} : constr subst_syn T := [{subst_syn,T}> 1 | tt, [*]].
-
-Definition empty_ctxt {T} := [{subst_syn,T}> 2 | tt, [*]].
-Definition cons_ctxt {T} a b := [{subst_syn,T}> 3 | tt, [* a; b]].
-
-Definition judg {T} c t := [{subst_syn,T}> 4 | tt, [* c; t]].
-
-Definition zv {T} := [{subst_syn,T}> 5 | tt, [*]].
-Definition sv {T} x := [{subst_syn,T}> 6 | tt, [* x]].
-
-Definition empty_sub {T} := [{subst_syn,T}> 7 | tt, [*]].
-Definition cons_sub {T} a b := [{subst_syn,T}> 8 | tt, [* a; b]].
-
-Definition tp' := [{subst_syn} 0 | tt, [*]].
-Definition ctxt' := [{subst_syn} 1 | tt, [*]].
-
-Definition empty_ctxt' := [{subst_syn} 2 | tt, [*]].
-Definition cons_ctxt' a b := [{subst_syn} 3 | tt, [* a; b]].
-
-Definition judg' c t := [{subst_syn} 4 | tt, [* c; t]].
-
-Definition zv' := [{subst_syn} 5 | tt, [*]].
-Definition sv' x := [{subst_syn} 6 | tt, [* x]].
-
-Definition empty_sub' := [{subst_syn} 7 | tt, [*]].
-Definition cons_sub' a b := [{subst_syn} 8 | tt, [* a; b]].
-
-Definition var_srt' s :=  [{subst_syn} 9 | tt, [* s]].
-
-Notation "@!" := empty_ctxt'.
-Notation "C ,, t" := (cons_ctxt' C t) (at level 90).
-
-
-
-
-Lemma wf_subst_lang : wf_lang subst_lang.
-Proof.
-  unfold subst_lang.
-  constructor; constructor.
-  constructor.
-  constructor; constructor.
-  - constructor; constructor.
-    change ctxt
-    eapply wf_sort_subst.
-    constructor.
-    Focus 2.
-    simpl.
-    eauto.
-
-  eauto.
-  constructor.
-  - repeat constructor.
-
-  simpl; eauto.
-  constructor.
-     (* TODO: how to talk about an arbitrary coefficient? needs to be 3rd ctxt option? *)
-     {| [:: coeff] |- (svar' 0) .: judg' (@! ,, (var 0)) (var 0)}].
-
-                                                                  
